fairness/heap_lang/execution_model.v
@@ -1,0 +1,7 @@
+From stdpp Require Import fin_maps.
+From iris.proofmode Require Import tactics.
+(* From trillium.program_logic Require Export weakestpre adequacy. *)
+(* From trillium.fairness Require Export fairness. *)
+From trillium.fairness.heap_lang Require Export lang.
+
+
